add iInduction

eIris/proofmode/intros.v
@@ -1,16 +1,18 @@
 From elpi Require Import elpi.
 From iris.proofmode Require Export tactics coq_tactics reduction.
 From iris.prelude Require Import options.
-From iris.bi Require Export bi telescopes.
+From iris.bi Require Export bi.
+From iris.algebra Require Import ofe monoid list.
 
-From eIris.proofmode Require Import base reduction.
+From eIris.proofmode Require Import base reduction inductiveDB inductive.
 From eIris.proofmode.elpi Extra Dependency "iris_ltac.elpi" as iris_ltac.
 From eIris.proofmode.elpi Extra Dependency "eiris_tactics.elpi" as eiris_tactics.
 
-From iris.heap_lang Require Import proofmode.
+From iris.heap_lang Require Import proofmode notation.
 
 Elpi Tactic eiIntros.
 Elpi Accumulate Db reduction.db.
+Elpi Accumulate Db induction.db.
 Elpi Accumulate File eiris_tactics.
 Elpi Accumulate lp:{{
   shorten coq.ltac.{ open, thenl, all }.
@@ -22,8 +24,7 @@ Elpi Accumulate lp:{{
   parse_args [str Args] IPS :- !,
     tokenize Args T, !,
     parse_ipl T IPS.
-  parse_args _ _ :-
-    coq.say Args,
+  parse_args Args _ :-
     coq.ltac.fail 0 "Did not recognize arguments" Args.
 
   solve (goal _ _ Type Proof [str "debug" | Args]) GS :-
@@ -47,22 +48,199 @@ Elpi Accumulate lp:{{
 }}.
 Elpi Typecheck.
 
+Elpi Tactic eiDestruct.
+Elpi Accumulate Db reduction.db.
+Elpi Accumulate Db induction.db.
+Elpi Accumulate File eiris_tactics.
+Elpi Accumulate lp:{{
+  shorten coq.ltac.{ open, thenl, all }.
 
-Tactic Notation "eiIntros" :=
-  elpi eiIntros asdfasf.
+  pred parse_destruct_args i:list argument, o:ident, o:intro_pat.
+  parse_destruct_args [str IDS, str Args] (iNamed IDS) IP :- !,
+    tokenize Args T, !,
+    parse_ipl T [IP].
+  parse_destruct_args Args _ _ :-
+    coq.ltac.fail 0 "Did not recognize arguments" Args.
 
-Tactic Notation "eiIntros" "(" simple_intropattern_list(l) ")" :=
-  elpi eiIntros ltac_tactic:( intros l ) "".
+  solve (goal _ _ Type Proof [str "debug" | Args]) GS :-
+    gettimeofday Start,
+    [get-option "debug" tt, get-option "start" Start] => (
+      parse_destruct_args Args ID IP, !,
+      do-iStartProof (hole Type Proof) IH, !,
+      do-iDestruct ID IP IH (ih\ set-ctx-count-proof ih _), !,
+      coq.ltac.collect-goals Proof GL SG,
+      all (open pm-reduce-goal) GL GL',
+      all (open show-goal) GL' _,
+      std.append GL' SG GS
+    ).
+  solve (goal _ _ Type Proof Args) GS :-
+    parse_destruct_args Args ID IP, !,
+    do-iStartProof (hole Type Proof) IH, !,
+    do-iDestruct ID IP IH (ih\ set-ctx-count-proof ih _), !,
+    coq.ltac.collect-goals Proof GL SG,
+    all (open pm-reduce-goal) GL GL',
+    std.append GL' SG GS.
+}}.
+Elpi Typecheck.
+
+Elpi Tactic eiInduction.
+Elpi Accumulate Db reduction.db.
+Elpi Accumulate Db induction.db.
+Elpi Accumulate File eiris_tactics.
+Elpi Accumulate lp:{{
+  shorten coq.ltac.{ open, thenl, all }.
+
+  pred do-iInduction i:ident, i:intro_pat, i:ihole, o:(ihole -> prop).
+  do-iInduction ID IP (ihole _ (hole Type _) as IH) C :-
+    find-hyp ID Type (app [global GREF | Args]),
+    inductive-ind GREF INDLem, !,
+    if-debug (coq.say "Induction on" INDLem Args),
+    inductive-type GREF T, !,
+    if-debug (coq.say "with Type" T),
+    do-iInduction.inner ID IP T (app [global INDLem]) Args IH C.
+
+  pred do-iInduction.inner i:ident, i:intro_pat, i:indt-decl, i:term, i:list term, i:ihole, o:(ihole -> prop).
+  do-iInduction.inner ID IP (inductive _Name _In-Or-Co Arity Constructors) (app INDLem) Args (ihole _ (hole Type _) as IH) C :-
+    Type = {{ envs_entails _ lp:P }},
+    std.map Args (x\r\ sigma N T I\ decl x N T, coq.name->id N I, r = par I _ T x ) Pars, !,
+    replace-params-bo Pars P Phi, !,
+    if-debug (coq.say "phi is" Phi),
+    Lem = app {std.append INDLem [Phi]},
+    if-debug (coq.say "Lem to apply" Lem),
+    % Apply induction lemma
+    do-iApplyLem Lem IH [] [IntroIH, IHyp],
+    % Apply induction hyp to goal
+    do-iApplySimpleExact IHyp ID,
+    % Introduce created goal
+    std.map {std.iota {type-depth {coq.arity->term Arity} } } (x\r\ r = iPure none) Pures,
+    (pi f\ std.length (Constructors f) NConstr),
+    if (IP = iAll) (
+        IP' = iList {std.map {std.iota NConstr} (x\r\ r = [iFresh])}
+      ) (IP' = IP),
+    do-iIntros {std.append [iModalIntro| Pures] [IP']} IntroIH C.
+  do-iInduction.inner HID IP (parameter _ _ _ IND) (app INDLem) [A | Args] IH C :-
+    pi p\ do-iInduction.inner HID IP (IND p) (app {std.append INDLem [A]}) Args IH C.
+
+
+  pred parse_destruct_args i:list argument, o:ident, o:intro_pat.
+  parse_destruct_args [str IDS, str Args] (iNamed IDS) IP :- !,
+    tokenize Args T, !,
+    parse_ipl T [IP].
+  parse_destruct_args Args _ _ :-
+    coq.ltac.fail 0 "Did not recognize arguments" Args.
+
+  solve (goal _ _ Type Proof [str "debug" | Args]) GS :- !,
+    gettimeofday Start,
+    [get-option "debug" tt, get-option "start" Start] => (
+      parse_destruct_args Args ID IP, !,
+      do-iStartProof (hole Type Proof) IH, !,
+      do-iInduction ID IP IH (ih\ set-ctx-count-proof ih _), !,
+      if-debug (coq.say "Induction done"),
+      coq.ltac.collect-goals Proof GL SG, !,
+      all (open pm-reduce-goal) GL GL', !,
+      all (open show-goal) GL' _, !,
+      std.append GL' SG GS
+    ).
+  solve (goal _ _ Type Proof Args) GS :-
+    parse_destruct_args Args ID IP, !,
+    do-iStartProof (hole Type Proof) IH, !,
+    do-iInduction ID IP IH (ih\ set-ctx-count-proof ih _), !,
+    coq.ltac.collect-goals Proof GL SG,
+    all (open pm-reduce-goal) GL GL',
+    std.append GL' SG GS.
+}}.
+Elpi Typecheck.
 
 Tactic Notation "eiIntros" string(x) :=
   elpi eiIntros ltac_string:(x).
 
-Tactic Notation "eiIntros" "(" simple_intropattern_list(l) ")" string(x) :=
-  elpi eiIntros ltac_tactic:( intros l ) ltac_string:(x).
+Tactic Notation "eiDestruct" string(x) "as" string(y) :=
+  elpi eiDestruct debug ltac_string:(x) ltac_string:(y).
+
+Tactic Notation "eiDestruct" string(x) :=
+  elpi eiDestruct debug ltac_string:(x) "**".
+
+Tactic Notation "eiInduction" string(x) "as" string(y) :=
+  elpi eiInduction debug ltac_string:(x) ltac_string:(y).
+
+Tactic Notation "eiInduction" string(x) :=
+  elpi eiInduction debug ltac_string:(x) "**".
 
 Section Proof.
   Context `{!heapGS Σ}.
   Notation iProp := (iProp Σ).
+  Implicit Types l : loc.
+
+  (* #[debug]
+  EI.ind 
+  Inductive is_list_alt (q : Qp) : val → list val → iProp :=
+    | empty_is_list : is_list_alt q NONEV []
+    | empty_alt_is_list : is_list_alt q NONEV [NONEV]
+    | cons_is_list l v vs tl : l ↦{#q} (v,tl) -∗ is_list_alt q tl vs -∗ is_list_alt q (SOMEV #l) (v :: vs). *)
+
+  (* Lemma intros_ind (q : Qp) (v : val) (vs : list val) :
+    is_list_alt q v vs -∗ is_list_alt q v vs.
+  Proof.
+    eiIntros "H".
+    eiDestruct "H"; iApply is_list_alt_unfold_2.
+    + by iLeft.
+    + iRight. by iLeft.
+    + iRight. by iRight.
+  Qed. *)
+
+  EI.ind 
+  Inductive is_list (q : Qp) : val → list val → iProp :=
+    | empty_is_list : is_list q NONEV []
+    | cons_is_list l v vs tl : l ↦{#q} (v,tl) -∗ is_list q tl vs -∗ is_list q (SOMEV #l) (v :: vs).
+
+  Print is_list_pre.
+
+  Lemma ind_test_1 (q q' : Qp) (v : val) (vs : list val) :
+    is_list q v vs ∗ is_list q' v vs ∗-∗ is_list (q+q') v vs.
+  Proof.
+    iSplit.
+    - eiIntros "[Hq Hq']".
+      iRevert "Hq'".
+      eiInduction "Hq" as "[IH|IH]"; eiIntros "Hq'".
+      + iApply is_list_unfold_2.
+        iLeft.
+        iFrame.
+      + eiDestruct "IH" as "[%l' [%v' [%vs' [%tl' (Hl' & IH & %Hx & %Hy)]]]]". 
+        simplify_eq.
+        iApply is_list_unfold_2.
+        iRight.
+        iExists l', v', vs', tl'.
+        eiDestruct "Hq'" as "[[%Hl %Hv] | [%l'' [%v'' [%vs'' [%tl'' (Hl & Hilq' & %Hl & %Hv)]]]]]"; simplify_eq.
+        iCombine "Hl' Hl" as "Hl" gives %[_ ?]; simplify_eq.
+        iFrame.
+        iDestruct "IH" as "[IH _]".
+        iSplitL.
+        * iApply ("IH" with "[$]").
+        * iSplit; iPureIntro; done.
+    - eiIntros "Hi".
+      eiInduction "Hi" as "[IH|IH]".
+      + iDestruct "IH" as "[-> ->]".
+        iSplitL.
+        * iApply is_list_unfold.
+          iLeft.
+          by iPureIntro.
+        * iApply is_list_unfold.
+          iLeft.
+          by iPureIntro.
+      + eiDestruct "IH" as "[%l [%v' [%vs' [%tl ([Hq Hq'] & [[Hiq Hiq'] _] & %Hx & %Hy)]]]]".
+        iSplitL "Hq Hiq".
+        * iApply is_list_unfold.
+          iRight.
+          iExists l, v', vs', tl.
+          iFrame.
+          by iPureIntro.
+        * iApply is_list_unfold.
+          iRight.
+          iExists l, v', vs', tl.
+          iFrame.
+          by iPureIntro.
+  Qed.
+
 
   (* Elpi Trace Browser. *)
   Lemma intros_1 (Q : Prop) (P : nat -> iProp) :
