eIris/proofmode/inductive.v
@@ -1,469 +1,32 @@
 From elpi Require Import elpi.
 From iris.proofmode Require Import base environments proofmode tactics coq_tactics reduction intro_patterns class_instances spec_patterns.
 From iris.prelude Require Import options.
-From iris.bi Require Import  bi telescopes fixpoint.
+From iris.bi Require Import  bi.
 From iris.algebra Require Import ofe monoid list.
-From iris.heap_lang Require Import proofmode.
-From iris.heap_lang Require Import notation.
+From iris.heap_lang Require Import proofmode notation.
 From stdpp Require Import base finite.
 
 From eIris.proofmode Require Export proper.
 From eIris.proofmode Require Import reduction.
 From eIris.proofmode Require Import inductiveDB.
-
-From eIris.proofmode Require Import base intros apply startProof.
-From eIris.proofmode.elpi Extra Dependency "proper_solver.elpi" as proper_solver.
+From eIris.proofmode Require Import base.
+(* From eIris.proofmode Require Import intros apply startProof. *)
+From eIris.proofmode.elpi Extra Dependency "mk_inductive.elpi" as mkinductive.
 
 #[arguments(raw)] Elpi Command EI.ind.
 Elpi Accumulate Db reduction.db.
 Elpi Accumulate Db induction.db.
-Elpi Accumulate File proper_solver.
+Elpi Accumulate File mkinductive.
 Elpi Accumulate lp:{{
-  kind param type.
-  type par id -> implicit_kind -> term -> term -> param.
-
-  
-  pred constructor->term i:indc-decl, o:term.
-  constructor->term (constructor _ Arity) T :- coq.arity->term Arity T.
-
-
-  pred type-depth i:term, o:int.
-  type-depth (prod _ _ F) N :- !,
-    (pi x\ type-depth (F x) N'),
-    N is N' + 1.
-  type-depth _ 0.
-
-  
-  pred find-PROP i:term, o:term.
-  find-PROP (prod _ _ F) O :- !,
-    (pi x\ find-PROP (F x) O).
-  find-PROP O O :- !.
-
-  
-  pred type-to-fun i:term, o:term.
-  type-to-fun (prod N T F) (fun N T FB) :- !,
-    (pi x\ type-to-fun (F x) (FB x)).
-  type-to-fun X X :- !.
-
-  
-  pred init-prod-to-bi-exist i:term, o:term.
-  init-prod-to-bi-exist (prod N T F) {{ bi_exist lp:Fun}} :- !,
-    (pi x\ init-prod-to-bi-exist (F x) (F' x)),
-    Fun = (fun N T F').
-  init-prod-to-bi-exist X X.
-
-  
-  pred last-rec-to-and i:term, i:list term, i:term, o:term.
-  last-rec-to-and A B {{ bi_exist lp:{{ fun N T F}} }} {{ bi_exist lp:{{ fun N T F' }} }} :- !,
-    (pi x\ last-rec-to-and A B (F x) (F' x)).
-  last-rec-to-and A B {{ bi_sep lp:L lp:R }} {{ bi_sep lp:L lp:R' }} :- !,
-    last-rec-to-and A B R R'.
-  last-rec-to-and A B {{ bi_or lp:L lp:R }} {{ bi_or lp:L' lp:R' }} :- !,
-    last-rec-to-and A B L L',
-    last-rec-to-and A B R R'.
-  last-rec-to-and F [] (app [F]) {{ True }}.
-  last-rec-to-and F [L | LS] (app [F, T | TS]) TS' :-
-    {std.length LS} = {std.length TS}, !,
-    std.fold2 LS TS {{ (⌜lp:L = lp:T⌝)%I }} (l\ t\ a\ r\ sigma TMP\ TMP = {{ (⌜lp:l = lp:t⌝)%I }}, r = {{ (lp:a ∗ lp:TMP)%I }}) TS'.
-  last-rec-to-and _ [_ | _] (app [T | TS]) _ :-
-    coq.error "EI.Ind: " {coq.term->string (app [T | TS])} "has to many or to few arguments".
-
-  
-  pred top-wand-to-sepand i:term, o:term.
-  top-wand-to-sepand {{ bi_emp_valid lp:T }} T' :- !,
-    top-wand-to-sepand T T'.
-  top-wand-to-sepand {{ bi_exist lp:{{ fun N T F}} }} {{ bi_exist lp:{{ fun N T F' }} }} :- !,
-    (pi x\ top-wand-to-sepand (F x) (F' x)).
-  top-wand-to-sepand {{ bi_forall lp:{{ fun N T F}} }} {{ bi_forall lp:{{ fun N T F' }} }} :- !,
-    (pi x\ top-wand-to-sepand (F x) (F' x)).
-  top-wand-to-sepand {{ bi_wand lp:L lp:R }} {{ bi_sep lp:L lp:R' }} :- !,
-    top-wand-to-sepand R R'.
-  top-wand-to-sepand {{ bi_sep lp:L lp:R }} {{ bi_sep lp:L lp:R' }} :- !,
-    top-wand-to-sepand R R'.
-  top-wand-to-sepand X X :- !.
-
-  
-  pred replace-params-bo i:list param, i:term, o:term.
-  replace-params-bo [] T T.
-  replace-params-bo [(par ID _IK Type C) | Params] Term (fun N Type FTerm) :-
-    coq.id->name ID N,
-    replace-params-bo Params Term Term',
-    (pi x\ (copy C x :- !) => copy Term' (FTerm x)).
-
-  
-  pred replace-params-ty i:list param, i:term, o:term.
-  replace-params-ty [] T T.
-  replace-params-ty [(par ID _IK PType C) | Params] Type (prod N PType FType) :-
-    coq.id->name ID N,
-    replace-params-ty Params Type Type',
-    (pi x\ (copy C x :- !) => copy Type' (FType x)).
-
-  
-  pred mk-constr-body-disj i:(term -> list indc-decl), o:int, o:(term -> term).
-  mk-constr-body-disj Constructors NConstr ConstrBo :-
-    if-debug ((pi x\ print-contructors (Constructors x))),
-    (pi f\ std.length (Constructors f) NConstr),
-    (pi f\ std.map (Constructors f)
-      (x\ r\ sigma TMP1 TMP2\ 
-        constructor->term x TMP1, 
-        init-prod-to-bi-exist TMP1 TMP2, 
-        top-wand-to-sepand TMP2 r) % You can't spill here otherwise the TMP1 and TMP2 will be bound in the outer scope.
-      (ConstrBiTerms f)),
-    if-debug ((pi f\ coq.say "------ Constructor Bi Terms" {std.map (ConstrBiTerms f) coq.term->string})),
-    (pi f\ std.fold 
-      { std.drop-last 1 (ConstrBiTerms f) } 
-      { std.last (ConstrBiTerms f) }
-      (x\ a\ r\ r = {{ bi_or lp:a lp:x }}) 
-      (ConstrBo f)),
-    if-debug (coq.say "------ Constructor body disjunction" {coq.term->string (ConstrBo {{ True }})}).
-
-  
-  pred mk-constr-body i:list param, i:term, i:(term -> list indc-decl), o:int, o:term, o:term.
-  mk-constr-body Params TypeTerm Constructors NConstr EBo Ty :-
-    find-PROP TypeTerm PROP,
-    mk-constr-body-disj Constructors NConstr ConstrBo,
-    (pi b\ (type-to-fun PROP b :- !) => type-to-fun TypeTerm (FunTerm b)),
-    (pi b\
-      % Save the variables of functions in a list
-      (pi N T T1 F F1 A \ fold-map (fun N T F) A (fun N T1 F1) A :- !,
-                                  fold-map T A T1 _, pi x\ fold-map (F x) [x | A] (F1 x) _) => 
-      % When we hit our placeholder for the function body we replace it with the function body with the last application replaced by equalities for the arguments
-      (pi L L' F B \ fold-map b L B L :- !, std.rev L [F | L'], last-rec-to-and F L' (ConstrBo F) B) => 
-          fold-map {{fun F : lp:TypeTerm => lp:{{ FunTerm b }} }} [] Bo _),
-    replace-params-bo Params Bo PBo,
-    if-debug (coq.say "------- Body" { coq.term->string PBo }),
-    replace-params-ty Params {{ lp:TypeTerm -> lp:TypeTerm }} Ty, !,
-    if-debug (coq.say "------- Type" { coq.term->string Ty }),
-    @keepunivs! => std.assert-ok! (coq.elaborate-skeleton PBo Ty EBo) "Type check body failed".
-
-  
-  pred mk-proper i:list param, i:term, i:term, o:term.
-  mk-proper Params F Type EBo :-
-    find-PROP Type PROP,
-    (pi N T F A T1 F1 A1 \ fold-map (prod N T F) A (prod N T1 F1) (some {{ (.> lp:A1)%i_signature }}) :-
-          fold-map T A T1 _, !, (pi x\ fold-map (F x) A (F1 x) (some A1))) =>
-      (pi A \ fold-map PROP A PROP (some {{ bi_wand }}) :- !) =>
-        fold-map Type none Type (some R),
-    std.map Params (x\r\ x = (par _ _ _ r)) Ps,
-    Fapp = app [F | Ps],
-    replace-params-ty Params {{ IProper (□> lp:R ==> lp:R) lp:Fapp }} Proper,
-    @keepunivs! => std.assert-ok! (coq.elaborate-skeleton Proper {{ Prop }} EBo) "Type check proper failed".
-
-  
-  pred proper-proof i:term, o:term.
-  proper-proof Proper Proof :-
-    coq.typecheck Proof Proper ok,
-    do-solve-proper (hole Proper Proof).
-
-  
-  pred mk-fixpoint.fun i:term, i:list param, i:term, i:term, i:list term, o:term.
-  mk-fixpoint.fun Pre Params Type (prod N T F) L (fun N T F') :-
-    @pi-decl N T x\ mk-fixpoint.fun Pre Params Type (F x) [x | L] (F' x).
-  mk-fixpoint.fun Pre Params Type _ RevL {{ bi_forall lp:F }} :-
-    std.rev RevL L,
-    coq.id->name "Φ" N,
-    F = fun N Type Forall,
-    @pi-decl N Type phi\ ( sigma AppPhi\ sigma Prem\
-      AppPhi = app [phi | L],
-      mk-fixpoint.forall Pre Params phi [] Type Prem,
-      Forall phi = {{ bi_wand (□ lp:Prem) lp:AppPhi }}
-    ).
-
-  
-  pred mk-fixpoint.forall i:term, i:list param, i:term, i:list term, i:term, o:term.
-  mk-fixpoint.forall Pre Params Phi Xs (prod N T F) {{ bi_forall lp:Fun }} :-
-    Fun = fun N T F',
-    pi x\ mk-fixpoint.forall Pre Params Phi [x | Xs] (F x) (F' x).
-  mk-fixpoint.forall Pre Params Phi RevXs _ {{ bi_wand lp:L lp:R }} :-
-    std.rev RevXs Xs,
-    std.map Params (x\r\ x = par _ _ _ r) Ps,
-    L = app { std.append [Pre | Ps] [Phi | Xs] },
-    R = app [Phi | Xs].
-
-  
-  pred mk-fixpoint i:list param, i:term, i:term, o:term.
-  mk-fixpoint Params Type Pre Fixpoint :-
-    mk-fixpoint.fun Pre Params Type Type [] Fixpoint',
-    replace-params-bo Params Fixpoint' Fixpoint,
-    if-debug (coq.say "----- Fixpoint Body" {coq.term->string Fixpoint}),
-    coq.typecheck Fixpoint _ D, 
-    if (D = ok) (true) (coq.error D).
-
-
-  pred mk-fix-toproof i:(list term -> list term -> term -> prop), i:list param, i:term, i:list term, i:list term, i:term, o:term.
-  mk-fix-toproof MK Params Pre Fixes Xs (prod N T F) (prod N T F') :-
-    @pi-decl N T x\ mk-fix-toproof MK Params Pre Fixes [x | Xs] (F x) (F' x).
-  mk-fix-toproof MK Params Pre Fixes RevXs _ Res :-
-    std.rev RevXs Xs,
-    std.map Params (x\r\ x = par _ _ _ r) Ps,
-    std.map Fixes (f\r\ sigma App\ std.append [Pre | Ps] [app [f | Ps] | Xs] App, r = app App) Unfolds,
-    std.map Fixes (f\r\ sigma App\ std.append Ps Xs App, r = app [f | App]) Folds,
-    MK Unfolds Folds Res.
-  
-
-  pred mk-unfold-2.proof i:int, i:int, i:term, i:term, i:hole.
-  mk-unfold-2.proof Ps N Proper Mono (hole Type Proof) :-
-    do-intros-forall (hole Type Proof) (mk-unfold-2.proof-1 Ps N Proper Mono).
-
-  pred mk-unfold-2.proof-1 i:int, i:int, i:term, i:term, i:hole.
-  mk-unfold-2.proof-1 Ps N Proper Mono H :-
-    do-iStartProof H IH', !,
-    if-debug (coq.say "started proof unfold_2" {ihole->string IH'}),
-    do-iIntros [iIdent (iNamed "HF"), iPure none, 
-                iIntuitionistic (iIdent (iNamed "HI")), 
-                iHyp "HI"] IH' (mk-unfold-2.proof-2 Ps N Proper Mono).
-
-  pred mk-unfold-2.proof-2 i:int, i:int, i:term, i:term, i:ihole.
-  mk-unfold-2.proof-2 Ps N Proper Mono IH :-
-    ((copy {{ @IProper }} {{ @iProper }} :- !) => copy Mono MonoiProper'),
-    type-to-fun MonoiProper' MonoiProper,
-    std.map {std.iota Ps} (x\r\ r = {{ _ }}) Holes, !,
-    do-iApplyLem (app [MonoiProper | Holes]) IH [(h\ sigma PType\ sigma PProof\ sigma List\ sigma Holes2\ !,
-      h = hole PType PProof,
-      std.iota Ps List,
-      std.map List (x\r\ r = {{ _ }}) Holes2,
-      coq.elaborate-skeleton (app [Proper | Holes2]) PType PProof D,
-      if (D = ok) (true) (if-debug (coq.say "IProper error" D), fail)
-    )] [IH1, IH2],
-    if-debug (coq.say "pre apply HF" {ihole->string IH2}), !,
-    do-iApplyHyp "HF" IH2 [], !,
-    std.map {std.iota N} (x\r\ r = iPure none) Pures, !,
-    do-iIntros {std.append [iModalIntro | Pures] [iIdent (iNamed "H"), iHyp "H", iModalIntro, iHyp "HI"]} IH1 (ih\ true).
-
-  pred mk-unfold-2 i:list param, i:term, i:term, i:term, i:term, i:term, o:hole.
-  mk-unfold-2 Params Pre Proper Mono Fix Type (hole ToProof Proof) :-
-    mk-fix-toproof (u\f\res\ sigma U\ sigma F\ u = [U], f = [F], res = {{ lp:U ⊢ lp:F }}) Params Pre [Fix] [] Type ToProof', !,
-    replace-params-ty Params ToProof' ToProof, !,
-    if-debug (coq.say "unfold 2:" {coq.term->string ToProof}),
-    mk-unfold-2.proof {std.length Params} {type-depth Type} Proper Mono (hole ToProof Proof).
-
-
-  pred mk-unfold-1.proof i:int, i:int, i:term, i:term, i:term, i:hole.
-  mk-unfold-1.proof Ps N Unfold2 Proper Mono (hole Type Proof) :-
-    do-intros-forall (hole Type Proof) (mk-unfold-1.proof-1 Ps N Unfold2 Proper Mono).
-
-  pred mk-unfold-1.proof-1 i:int, i:int, i:term, i:term, i:term, i:hole.
-  mk-unfold-1.proof-1 Ps N Unfold2 Proper Mono H :-
-    do-iStartProof H IH', !,
-    if-debug (coq.say "started proof unfold_1" {ihole->string IH'}),
-    std.map {std.iota N} (x\r\ r = iPure none) Pures, !,
-    do-iIntros { std.append [iIdent (iNamed "HF"), iHyp "HF", iModalIntro | Pures]
-                            [iIdent (iNamed "Hy")] } 
-               IH' (mk-unfold-1.proof-2 Ps N Unfold2 Proper Mono).
-               
-  pred mk-unfold-1.proof-2 i:int, i:int, i:term, i:term, i:term, i:ihole.
-  mk-unfold-1.proof-2 Ps N Unfold2 Proper Mono IH :-
-    ((copy {{ @IProper }} {{ @iProper }} :- !) => copy Mono MonoiProper'),
-    type-to-fun MonoiProper' MonoiProper,
-    std.map {std.iota Ps} (x\r\ r = {{ _ }}) Holes, !,
-    do-iApplyLem (app [MonoiProper | Holes]) IH [(h\ sigma PType\ sigma PProof\ sigma List\ sigma Holes2\ !,
-      h = hole PType PProof,
-      std.iota Ps List,
-      std.map List (x\r\ r = {{ _ }}) Holes2,
-      coq.elaborate-skeleton (app [Proper | Holes2]) PType PProof D,
-      if (D = ok) (true) (if-debug (coq.say "IProper error" D), fail)
-    )] [IH1, IH2],
-    do-iApplyHyp "Hy" IH2 [], !,
-    std.map {std.iota N} (x\r\ r = iPure none) Pures, !,
-    do-iIntros {std.append [iModalIntro | Pures] [iIdent (iNamed "HF")]} IH1 (mk-unfold-1.proof-3 Ps Unfold2).
-
-  pred mk-unfold-1.proof-3 i:int, i:term, i:ihole.
-  mk-unfold-1.proof-3 Ps Unfold2 IH :-
-    std.map {std.iota Ps} (x\r\ r = {{ _ }}) Holes, !,
-    do-iApplyLem (app [Unfold2 | Holes]) IH [] [AppliedIH], !,
-    do-iApplyHyp "HF" AppliedIH [].
-
-  pred mk-unfold-1 i:list param, i:term, i:term, i:term, i:term, i:term, i:term, o:hole.
-  mk-unfold-1 Params Unfold2 Pre Proper Mono Fix Type (hole ToProof Proof) :-
-    mk-fix-toproof (u\f\res\ sigma U\ sigma F\ u = [U], f = [F], res = {{ lp:F ⊢ lp:U }}) Params Pre [Fix] [] Type ToProof', !,
-    replace-params-ty Params ToProof' ToProof,!,
-    if-debug (coq.say "unfold 1:" {coq.term->string ToProof}),
-    mk-unfold-1.proof {std.length Params} {type-depth Type} Unfold2 Proper Mono (hole ToProof Proof),
-    if-debug (coq.say "unfold 1 done").
-
-
-  pred mk-unfold.proof i:int, i:term, i:term, i:hole.
-  mk-unfold.proof Ps Unfold1 Unfold2 (hole Type Proof) :-
-    do-intros-forall (hole Type Proof) (mk-unfold.proof-1 Ps Unfold1 Unfold2).
-
-  pred mk-unfold.proof-1 i:int, i:term, i:term, i:hole.
-  mk-unfold.proof-1 Ps Unfold1 Unfold2 H :-
-    do-iStartProof H (ihole N H'), !,
-    if-debug (coq.say "Started proof" {ihole->string (ihole N H')}),
-    do-iAndSplit H' H1 H2,
-    if-debug (coq.say "H1:" {ihole->string (ihole N H1)}),
-    if-debug (coq.say "H2:" {ihole->string (ihole N H2)}),
-    std.map {std.iota Ps} (x\r\ r = {{ _ }}) Holes1, !,
-    do-iApplyLem (app [Unfold1 | Holes1]) (ihole N H1) [] [], !,
-    std.map {std.iota Ps} (x\r\ r = {{ _ }}) Holes2, !,
-    do-iApplyLem (app [Unfold2 | Holes2]) (ihole N H2) [] [].
-
-  pred mk-unfold i:list param, i:term, i:term, i:term, i:term, i:term, o:hole.
-  mk-unfold Params Unfold1 Unfold2 Pre Fix Type (hole ToProof Proof) :-
-    mk-fix-toproof (u\f\res\ sigma U\ sigma F\ u = [U], f = [F], res = {{ lp:F ⊣⊢ lp:U }}) Params Pre [Fix] [] Type ToProof', !,
-    replace-params-ty Params ToProof' ToProof,!,
-    if-debug (coq.say "unfold:" {coq.term->string ToProof}),
-    mk-unfold.proof {std.length Params} Unfold1 Unfold2 (hole ToProof Proof),
-    if-debug (coq.say "unfold done").
-
-
-  pred mk-iter.toproof-inner-1 i:list param, i:term, i:term, i:list term, i:term, o:term.
-  mk-iter.toproof-inner-1 Params Pre Phi Xs (prod N T F) {{ bi_forall lp:Fun }} :-
-    Fun = fun N T F',
-    @pi-decl N T x\ mk-iter.toproof-inner-1 Params Pre Phi [x | Xs] (F x) (F' x).
-  mk-iter.toproof-inner-1 Params Pre Phi RevXs _ {{ bi_wand lp:L lp:R }} :-
-    std.rev RevXs Xs,
-    std.map Params (x\r\ x = par _ _ _ r) Ps,
-    L = app {std.append [Pre | Ps] [Phi | Xs]},
-    R = app [Phi | Xs].
-
-  pred mk-iter.toproof-inner-2 i:list param, i:term, i:term, i:list term, i:term, o:term.
-  mk-iter.toproof-inner-2 Params Fix Phi Xs (prod N T F) {{ bi_forall lp:Fun }} :-
-    Fun = fun N T F',
-    @pi-decl N T x\ mk-iter.toproof-inner-2 Params Fix Phi [x | Xs] (F x) (F' x).
-  mk-iter.toproof-inner-2 Params Fix Phi RevXs _ {{ bi_wand lp:L lp:R }} :-
-    std.rev RevXs Xs,
-    std.map Params (x\r\ x = par _ _ _ r) Ps,
-    L = app {std.append [Fix | Ps] Xs},
-    R = app [Phi | Xs].
-
-  pred mk-iter.toproof i:list param, i:term, i:term, i:term, o:term.
-  mk-iter.toproof Params Pre Fix Type (prod N Type F) :-
-    coq.id->name "Φ" N,
-    (pi phi\ mk-iter.toproof-2 Params Pre Fix Type phi (F phi)).
-  
-  pred mk-iter.toproof-2 i:list param, i:term, i:term, i:term, i:term, o:term.
-  mk-iter.toproof-2 Params Pre Fix Type Phi ToProof :-
-    mk-iter.toproof-inner-1 Params Pre Phi [] Type Assump,
-    mk-iter.toproof-inner-2 Params Fix Phi [] Type Prem,
-    ToProof = {{ (□ lp:Assump) -∗ lp:Prem }}.
-
-  pred mk-iter.proof i:int, i:hole.
-  mk-iter.proof N (hole Type Proof) :-
-    do-intros-forall (hole Type Proof) (mk-iter.proof-1 N).
-
-  pred mk-iter.proof-1 i:int, i:hole.
-  mk-iter.proof-1 N H :-
-    do-iStartProof H IH, !,
-    std.map { std.iota N } (x\r\ r = iPure none) Pures, !,
-    do-iIntros {std.append [iIntuitionistic (iIdent (iNamed "Hphi")) | Pures]
-                           [iIdent (iNamed "HF"), iHyp "HF", iHyp "Hphi"]}
-               IH (ih\ true).
-  
-  pred mk-iter i:list param, i:term, i:term, i:term, o:hole.
-  mk-iter Params Pre Fix Type (hole ToProof Proof) :- 
-    mk-iter.toproof Params Pre Fix Type ToProof', !,
-    replace-params-ty Params ToProof' ToProof, !,
-    if-debug (coq.say "iter to proof" {coq.term->string ToProof}), !,
-    mk-iter.proof {type-depth Type} (hole ToProof Proof),
-    if-debug (coq.say "iter proof finished").
-
-
-  pred mk-ind.toproof i:list param, i:term, i:term, i:term, o:term.
-  mk-ind.toproof Params Pre Fix Type (prod N Type F) :-
-    coq.id->name "Φ" N,
-    (pi phi\ mk-ind.toproof-2 Params Pre Fix Type phi (F phi)).
-  
-  pred mk-ind.toproof-2 i:list param, i:term, i:term, i:term, i:term, o:term.
-  mk-ind.toproof-2 Params Pre Fix Type Phi {{ (□ lp:L) -∗ lp:R }} :-
-    mk-ind.toproof-inner Params Pre Fix Phi [] Type Type L,
-    mk-iter.toproof-inner-2 Params Fix Phi [] Type R.
-
-  pred mk-ind.toproof-fun i:list param, i:term, i:term, i:list term, i:term, o:term.
-  mk-ind.toproof-fun Params Phi Fix Xs (prod N T F) (fun N T F') :-
-    pi x\ mk-ind.toproof-fun Params Phi Fix [x | Xs] (F x) (F' x).
-  mk-ind.toproof-fun Params Phi Fix RevXs _ Res :-
-    std.rev RevXs Xs,
-    std.map Params (x\r\ x = par _ _ _ r) Ps,
-    L = app [Phi | Xs],
-    R = app [Fix | {std.append Ps Xs}],
-    Res = {{ bi_and lp:L lp:R }}.
-
-  pred mk-ind.toproof-inner i:list param, i:term, i:term, i:term, i:list term, i:term, i:term, o:term.
-  mk-ind.toproof-inner Params Pre Fix Phi Xs Type (prod N T F) {{ bi_forall lp:Fun }} :-
-    Fun = fun N T F',
-    @pi-decl N T x\ mk-ind.toproof-inner Params Pre Fix Phi [x | Xs] Type (F x) (F' x).
-  mk-ind.toproof-inner Params Pre Fix Phi RevXs Type _ {{ bi_wand lp:L lp:R }} :-
-    std.rev RevXs Xs,
-    std.map Params (x\r\ x = par _ _ _ r) Ps,
-    mk-ind.toproof-fun Params Phi Fix [] Type IH,
-    L = app {std.append [Pre | Ps] [IH | Xs]},
-    R = app [Phi | Xs].
-
-  pred mk-ind.proof i:int, i:int, i:term, i:term, i:term, i:term, i:term, i:hole.
-  mk-ind.proof Ps N Unfold1 Unfold2 Proper Mono Iter (hole Type Proof) :-
-    do-intros-forall (hole Type Proof) (mk-ind.proof-1 Ps N Unfold1 Unfold2 Proper Mono Iter).
-  
-  pred mk-ind.proof-1 i:int, i:int, i:term, i:term, i:term, i:term, i:term i:hole.
-  mk-ind.proof-1 Ps N Unfold1 Unfold2 Proper Mono Iter H :-
-    do-iStartProof H IH, !,
-    std.map {std.iota N} (x\r\ r = iPure none) Pures, !,
-    do-iIntros {std.append [iIntuitionistic (iIdent (iNamed "Hmon")) | Pures] 
-                           [iIdent (iNamed "Hx"), iHyp "Hmon"]} IH (mk-ind.proof-2 Ps N Unfold1 Unfold2 Proper Mono Iter).
-
-  pred mk-ind.proof-2 i:int, i:int, i:term, i:term, i:term, i:term, i:term, i:ihole.
-  mk-ind.proof-2 Ps N Unfold1 Unfold2 Proper Mono Iter (ihole IN H) :-
-    do-iEvalIn (iNamed "Hx") H IH H1,
-    do-iApplyLem Unfold1 IH [] [], !,
-    % Apply Monotinicity
-    ((copy {{ @IProper }} {{ @iProper }} :- !) => copy Mono MonoiProper'),
-    type-to-fun MonoiProper' MonoiProper,
-    std.map {std.iota Ps} (x\r\ r = {{ _ }}) Holes, !,
-    do-iApplyLem (app [MonoiProper | Holes]) (ihole IN H1) [(h\ sigma PType\ sigma PProof\ sigma List\ sigma Holes'\ sigma PTypeString\ !,
-      h = hole PType PProof,
-      std.iota Ps List,
-      std.map List (x\r\ r = {{ _ }}) Holes',
-      coq.elaborate-skeleton (app [Proper | Holes']) PType PProof D,
-      if (D = ok) (true) (if-debug (coq.say "IProper error" D), fail)
-    )] [(ihole N2 H2), IH2], !,
-    do-iApplyHyp "Hx" IH2 [], !,
-    % Continue proof
-    do-iModIntro H2 H3,
-    do-iApplyLem Iter (ihole N2 H3) [] [IH3],
-    std.map {std.iota N} (x\r\ r = iPure none) Pures, !,
-    do-iIntros {std.append [iModalIntro | Pures] [iIdent (iNamed "Hilp")]} IH3 (mk-ind.proof-3 Ps N Unfold2 Proper Mono).
-
-  pred mk-ind.proof-3 i:int, i:int, i:term, i:term, i:term, i:ihole.
-  mk-ind.proof-3 Ps N Unfold2 Proper Mono (ihole IN H) :-
-    do-iAndSplit H H1 H2,!,
-    % Left branch
-    do-iApplyHyp "Hmon" (ihole IN H1) [IH1],!,
-    do-iApplyHyp "Hilp" IH1 [],!,
-    % Right branch
-    do-iApplyLem Unfold2 (ihole IN H2) [] [IH2],!,
-    % Apply Mono
-    ((copy {{ @IProper }} {{ @iProper }} :- !) => copy Mono MonoiProper'),
-    type-to-fun MonoiProper' MonoiProper,
-    std.map {std.iota Ps} (x\r\ r = {{ _ }}) Holes, !,
-    do-iApplyLem (app [MonoiProper | Holes]) IH2 [(h\ sigma PType\ sigma PProof\ sigma List\ sigma Holes'\ !,
-      h = hole PType PProof,
-      std.iota Ps List,
-      std.map List (x\r\ r = {{ _ }}) Holes',
-      coq.elaborate-skeleton (app [Proper | Holes']) PType PProof D,
-      if (D = ok) (true) (if-debug (coq.say "IProper error" D), fail)
-    )] [IH3, IH4],!,
-    do-iApplyHyp "Hilp" IH4 [], !,
-    std.map {std.iota N} (x\r\ r = iPure none) Pures, !,
-    do-iIntros {std.append [iModalIntro | Pures] [iList [[iDrop, iIdent (iNamed "Hilp")]], iHyp "Hilp"]} IH3 (ih\ true).
-
-  pred mk-ind i:list param, i:term, i:term, i:term, i:term, i:term, i:term, i:term, i:term, o:hole.
-  mk-ind Params Pre Fix Unfold1 Unfold2 Proper Mono Iter Type (hole ToProof Proof) :-
-    mk-ind.toproof Params Pre Fix Type ToProof',
-    replace-params-ty Params ToProof' ToProof, !,
-    if-debug (coq.say "ind to proof" {coq.term->string ToProof}), !,
-    mk-ind.proof {std.length Params} {type-depth Type} Unfold1 Unfold2 Proper Mono Iter (hole ToProof Proof), !,
-    if-debug (coq.say "ind proof finished").
-
-
-  pred create-iInductive i:list param, i:indt-decl.
-  create-iInductive Params' (inductive Name _In-Or-Co Arity Constructors) :-
+  pred create-iInductive i:list param, i:indt-decl, o:gref , o:indt-decl.
+  create-iInductive Params' (inductive Name In-Or-Co Arity Constructors) (const Fix) (inductive Name In-Or-Co Arity BIConstructors) :-
     std.rev Params' Params,
     if-debug (coq.say Params),
     if-debug (coq.say "------ Creating inductive" Name),
     coq.arity->term Arity TypeTerm,
     if-debug (coq.say "------ With type" { coq.term->string TypeTerm }),
 
-    mk-constr-body Params TypeTerm Constructors NConstr EBo Ty,
+    mk-constr-body Params TypeTerm Constructors NConstr BIConstructors EBo Ty,
     if-debug (coq.say "------ typed body" { coq.term->string EBo }),
     coq.env.add-const {calc (Name ^ "_pre")} EBo Ty ff C,
     if-debug (coq.say "const" C),!,
@@ -487,7 +50,7 @@ Elpi Accumulate lp:{{
       coq.env.add-const Name Fixpoint _ ff Fix,
       if-debug (coq.say "Fixpoint" Fix),
 
-      coq.elpi.accumulate _ "induction.db" (clause _ _ (inductive-pre (const Fix) (const C) NConstr)),
+      coq.elpi.accumulate _ "induction.db" (clause _ _ (inductive-pre (const Fix) (const C))),
       coq.elpi.accumulate _ "induction.db" (clause _ _ (inductive-mono (const Fix) (const M)))
       ),!,
 
@@ -503,7 +66,9 @@ Elpi Accumulate lp:{{
 
       mk-unfold Params (global (const U1)) (global (const U2)) (global (const C)) (global (const Fix)) TypeTerm (hole UnfoldType UnfoldProof),
       coq.env.add-const {calc (Name ^ "_unfold")} UnfoldProof UnfoldType ff U,
-      if-debug (coq.say "unfold" U)
+      if-debug (coq.say "unfold" U),
+
+      coq.elpi.accumulate _ "induction.db" (clause _ _ (inductive-unfold (const Fix) (const U1) (const U2) (const U) NConstr))
       ),!,
 
     if (get-option "noiter" tt) (true)
@@ -518,7 +83,6 @@ Elpi Accumulate lp:{{
     if (get-option "noind" tt) (true)
       (
       mk-ind Params (global (const C)) (global (const Fix)) (global (const U1)) (global (const U2)) (global (const M)) Proper (global (const IterConst)) TypeTerm (hole IndType IndProof), !,
-      % if-debug (coq.say "Pre add const" {coq.term->string IndType} {coq.term->string IndProof}),
       coq.ltac.collect-goals IndProof GS SGS,
       std.forall GS (x\ coq.ltac.open show-goal x _),
       std.forall SGS (x\ coq.ltac.open show-goal x _),
@@ -527,11 +91,9 @@ Elpi Accumulate lp:{{
 
       coq.elpi.accumulate _ "induction.db" (clause _ _ (inductive-ind (const Fix) (const IndConst)))
       ).
-  create-iInductive Params (parameter ID IK T IND) :-
+  create-iInductive Params (parameter ID IK T IND) Fix (parameter ID IK T IND') :-
     coq.id->name {calc (ID ^ "_param")} N,
-    @pi-decl N T p\ create-iInductive [(par ID IK T p) | Params] (IND p).
-    % pi p\ create-iInductive [(par ID IK T p) | Params] (IND p).
-
+    @pi-decl N T p\ create-iInductive [(par ID IK T p) | Params] (IND p) Fix (IND' p).
 
   main [indt-decl I] :- 
     attributes A,
@@ -547,26 +109,13 @@ Elpi Accumulate lp:{{
     gettimeofday Start,
     [get-option "start" Start | Opts] => (
       if (get-option "noproper" tt, not (get-option "nosolver" tt)) (coq.error "Can't do solver when noproper") (true),
-      create-iInductive [] I
-      ).
+      create-iInductive [] I Fix I',
+      if-debug (coq.say "saving type" Fix I'),
+      coq.elpi.accumulate _ "induction.db" (clause _ _ (inductive-type Fix I'))
+    ).
 }}.
 Elpi Typecheck.
-
 Elpi Export EI.ind.
-
-(* Elpi Tactic IProper_solver.
-Elpi Accumulate Db reduction.db.
-Elpi Accumulate File proper_solver.
-Elpi Accumulate lp:{{
-  solve (goal _Ctx _Trigger Type Proof []) _ :- 
-    do-solve-proper (hole Type Proof).
-  
-  solve (goal _Ctx _Trigger Type Proof [str "debug"]) _ :- 
-    gettimeofday Start,
-    [get-option "debug" tt, get-option "start" Start] => do-solve-proper (hole Type Proof).
-}}.
-Elpi Typecheck.
-Elpi Export IProper_solver. *)
 
 (* Implicit Types l : loc.
 
@@ -600,123 +149,6 @@ Section Tests.
   (* islist q -> [] ∨ q <= 1 *)
   (* islist (DfracOwn q) -> |==> islist (DfracDiscarded) *)
   (* Pers islist DfracDiscarded *)
-
-  (* Lemma least_fixpoint_ind_ei (q : Qp) (Φ : val → list val → iProp) :
-    □ (∀ x y, is_list_pre q (λ x' y', Φ x' y' ∧ is_list q x' y') x y -∗ Φ x y) -∗
-    ∀ x y, is_list q x y -∗ Φ x y.
-  Proof using Type*.
-    eiIntros "#Hmon % %".
-    eiIntros "Hx @Hmon".
-
-    notypeclasses refine (tac_eval_in _ "Hx" _ _ _ _ _ _ _).
-    1: {
-      pm_reflexivity.
-    }
-    1: {
-      pm_reduce.
-      eiStartProof.
-      1: iApply is_list_unfold_1.
-    }
-    pm_reduce.
-
-    iApply (iProper (□> .> .> bi_wand ==> .> .> bi_wand) (is_list_pre q)).
-    { apply is_list_pre_mono. }
-    2: { iApply "Hx". }
-    eiIntros "!>".
-    iApply is_list_iter.
-    eiIntros "!> % % Hilp".
-    iSplit.
-    - eiIntros "@Hmon @Hilp".
-    - iApply is_list_unfold_2.
-      iApply (iProper (□> .> .> bi_wand ==> .> .> bi_wand) (is_list_pre q)).
-      { apply is_list_pre_mono. }
-      2: { iApply "Hilp". }
-      eiIntros "!> % % [_ Hilp] @Hilp".
-  Qed. *)
-(* 
-  Lemma least_fixpoint_ind (q : Qp) (Φ : val → list val → iProp) :
-    □ (∀ x y, is_list_pre q (λ x' y', Φ x' y' ∧ is_list q x' y') x y -∗ Φ x y) -∗
-    ∀ x y, is_list q x y -∗ Φ x y.
-  Proof using Type*.
-    iIntros "#Hmon" (x y).
-    rewrite is_list_unfold_1.
-    iIntros "Hx".
-    eiIntros "@Hmon".
-    iApply (iProper (□> .> .> bi_wand ==> .> .> bi_wand) (is_list_pre q)).
-    { apply is_list_pre_mono. }
-    2: { iApply "Hx". }
-    iModIntro.
-    iApply is_list_iter.
-    iIntros "!>" (a b) "Hilp".
-    iSplit.
-    - iApply "Hmon". iApply "Hilp".
-    - iApply is_list_unfold_2.
-      iApply (iProper (□> .> .> bi_wand ==> .> .> bi_wand) (is_list_pre q)).
-      { apply is_list_pre_mono. }
-      2: { iApply "Hilp". }
-      iIntros "!>" (c d) "Hilp".
-      iDestruct "Hilp" as "[_ $]".
-  Qed. *)
-
-  Lemma ind_test_1 (q q' : Qp) (v : val) (vs : list val) :
-    is_list q v vs ∗ is_list q' v vs ∗-∗ is_list (q+q') v vs.
-  Proof.
-    iSplit.
-    - eiIntros "[Hq Hq']".
-      iRevert "Hq'".
-      iApply (is_list_ind q (λ v vs, is_list q' v vs -∗ is_list (q + q') v vs)%I with "[] Hq").
-      iIntros "!> %x %y [IH|IH]"; iIntros "Hq'".
-      + iDestruct "IH" as "[%l' [%v' [%vs' [%tl' (Hl' & IH & %Hx & %Hy)]]]]". 
-        simplify_eq.
-        iApply is_list_unfold_2.
-        iLeft.
-        iExists l', v', vs', tl'.
-        (* iPoseProofCore (is_list_unfold _ _ _) as true (fun Heq => idtac Heq;
-        eapply (tac_rewrite_in _ Heq _ _ "Hq'" _ _ Right)).
-        1: {
-          pm_reflexivity.
-        }
-        1: {
-          pm_reflexivity.
-        }
-        1: {
-          tc_solve || let P := match goal with |- IntoInternalEq ?P _ _ => P end in fail "iRewrite:" P "not an equality".
-          
-        } *)
-        (* iRewrite is_list_unfold in "Hq'". *)
-        iEval (rewrite is_list_unfold) in "Hq'".
-        iDestruct "Hq'" as "[[%l'' [%v'' [%vs'' [%tl'' (Hl & Hilq' & %Hl & %Hv)]]]] | [%Hl %Hv]]"; simplify_eq.
-        iCombine "Hl' Hl" as "Hl" gives %[_ ?]; simplify_eq.
-        iFrame.
-        admit.
-      + iApply is_list_unfold_2.
-        unfold is_list_pre.
-        iRight.
-        iFrame.
-    - eiIntros "Hi".
-      iApply (least_fixpoint_ind _ (λ v vs, is_list q v vs ∗ is_list q' v vs)%I with "[] Hi").
-      iIntros "!> %x %y [IH|IH]".
-      + iDestruct "IH" as "[%l [%v' [%vs' [%tl ([Hq Hq'] & [[Hiq Hiq'] _] & %Hx & %Hy)]]]]".
-        iSplitL "Hq Hiq".
-        * iApply is_list_unfold.
-          iLeft.
-          iExists l, v', vs', tl.
-          iFrame.
-          by iPureIntro.
-        * iApply is_list_unfold.
-          iLeft.
-          iExists l, v', vs', tl.
-          iFrame.
-          by iPureIntro.
-      + iDestruct "IH" as "[-> ->]".
-        iSplitL.
-        * iApply is_list_unfold.
-          iRight.
-          by iPureIntro.
-        * iApply is_list_unfold.
-          iRight.
-          by iPureIntro.
-  Admitted.
 
   EI.ind 
   Inductive is_l : val → iProp :=
