eIris/proofmode/startProof.v
@@ -2,13 +2,14 @@ From elpi Require Import elpi.
 From iris.proofmode Require Export tactics coq_tactics reduction.
 From iris.prelude Require Import options.
 
-From eIris.proofmode Require Import base reduction.
+From eIris.proofmode Require Import base reduction inductiveDB.
 From eIris.proofmode.elpi Extra Dependency "eiris_tactics.elpi" as eiris_tactics.
 
 From iris.heap_lang Require Import proofmode.
  
 Elpi Tactic eiStartProof.
 Elpi Accumulate Db reduction.db.
+Elpi Accumulate Db induction.db.
 Elpi Accumulate File eiris_tactics.
 Elpi Accumulate lp:{{
   solve (goal _ _ Type Proof _) _ :-
